%% LyX 2.3.4.2 created this file.  For more info, see http://www.lyx.org/.
%% Do not edit unless you really know what you are doing.
\documentclass[english]{article}
\usepackage[T1]{fontenc}
\usepackage[latin9]{inputenc}
\usepackage{amstext}
\usepackage{esint}
\usepackage{babel}
\begin{document}
\[
ds\ast dA\ast\frac{\text{rate of energy absorbed}}{\text{volume}}=(I\vert_{s}-I\vert_{s+ds})dA
\]

\[
\int_{I_{\lambda}e^{\tau_{\lambda}}\vert_{\tau_{\lambda}=0}}^{I_{\lambda}e^{\tau_{\lambda}}\vert_{\tau_{\lambda}=\tau_{\lambda}}}(dI_{\lambda}e^{\tau_{\lambda}})=\int_{\tau_{\lambda}=0}^{\tau_{\lambda}=\tau_{\lambda}}S(\tau_{\lambda},\hat{s})e^{\tau_{\lambda}}d\tau_{\lambda}
\]

\[
\frac{\partial I_{1}}{\partial\tau_{\lambda}}=\frac{\partial}{\partial\tau_{\lambda}}(2\pi\int_{-1}^{1}\mu I_{\lambda}(\tau_{\lambda})d\mu)
\]

\[
\frac{\partial I_{1}}{\partial\tau_{\lambda}}=2\pi(\int_{-1}^{1}\mu\frac{\partial}{\partial\tau_{\lambda}}I_{\lambda}(\tau_{\lambda})d\mu)
\]


\part{OpenFOAM Radiation Models}

\section{Spherical Harmonics Basic Concepts}

\subsection{Expanding out the Intensity Field}

\[
I(r,\hat{s})=\sum_{l=0}^{\infty}\sum_{m=-l}^{l}I_{l}^{m}(r)Y_{l}^{m}(\hat{s})
\]

Let's try writing out from l=0 to l=3

\medskip{}


\subsubsection{l=0 (1 term)}

\[
I(r,\hat{s})(l=0)=\sum_{m=-0}^{0}I_{0}^{m}(r)Y_{0}^{m}(\hat{s})=I_{0}^{0}(r)Y_{0}^{0}(\hat{s})
\]


\subsubsection{l=1 (3 terms)}

\[
I(r,\hat{s})(l=1)=\sum_{m=-1}^{1}I_{1}^{m}(r)Y_{1}^{m}(\hat{s})
\]

\[
=I_{1}^{-1}(r)Y_{1}^{-1}(\hat{s})+I_{1}^{0}(r)Y_{1}^{0}(\hat{s})+I_{1}^{1}(r)Y_{1}^{1}(\hat{s})
\]


\subsubsection{l=2 (5 terms)}

\[
I(r,\hat{s})(l=2)=\sum_{m=-2}^{2}I_{2}^{m}(r)Y_{2}^{m}(\hat{s})
\]

\[
=I_{2}^{-2}(r)Y_{2}^{-2}(\hat{s})+I_{2}^{-1}(r)Y_{2}^{-1}(\hat{s})+I_{2}^{0}(r)Y_{2}^{0}(\hat{s})+I_{2}^{1}(r)Y_{2}^{1}(\hat{s})+I_{2}^{2}(r)Y_{2}^{2}(\hat{s})
\]


\subsubsection{l=3 (7 terms)}

\[
I(r,\hat{s})(l=3)=\sum_{m=-3}^{3}I_{3}^{m}(r)Y_{3}^{m}(\hat{s})
\]

\[
=I_{3}^{-2}(r)Y_{3}^{-2}(\hat{s})+I_{3}^{-1}(r)Y_{3}^{-1}(\hat{s})+I_{3}^{0}(r)Y_{3}^{0}(\hat{s})+I_{3}^{1}(r)Y_{3}^{1}(\hat{s})+I_{3}^{2}(r)Y_{3}^{2}(\hat{s})
\]

\[
+I_{3}^{-3}(r)Y_{3}^{-3}(\hat{s})+I_{3}^{-3}(r)Y_{3}^{-3}(\hat{s})
\]


\subsection{Legendre's ODE}

\[
\frac{1}{\Theta(\theta)}\frac{\partial^{2}\Theta(\theta)}{\partial\theta^{2}}=\frac{1}{\Theta(\theta)}(\sin^{2}\theta\frac{\partial^{2}\Theta(x)}{\partial x^{2}}+\sin\theta\frac{\partial\Theta(x)}{\partial x}\frac{\text{\ensuremath{\partial\sin\theta}}}{\partial x})
\]

\[
\frac{1}{\Theta(\theta)}\frac{\partial^{2}\Theta(\theta)}{\partial\theta^{2}}=\frac{1}{\Theta(\theta)}(\sin^{2}\theta\frac{\partial^{2}\Theta(x)}{\partial x^{2}}+\sin\theta\frac{\partial\Theta(x)}{\partial x}\frac{\text{-\ensuremath{\cos}\ensuremath{\theta}}}{\sin\theta})
\]

\[
\frac{1}{\Theta(\theta)}\frac{\partial^{2}\Theta(\theta)}{\partial\theta^{2}}=\frac{1}{\Theta(\theta)}(\sin^{2}\theta\frac{\partial^{2}\Theta(x)}{\partial x^{2}}+-\cos\theta\frac{\partial\Theta(x)}{\partial x})
\]

In terms of x

\[
\frac{1}{\Theta(\theta)}\frac{\partial^{2}\Theta(\theta)}{\partial\theta^{2}}=\frac{1}{\Theta(\theta)}((1-x^{2})\frac{\partial^{2}\Theta(x)}{\partial x^{2}}+-x\frac{\partial\Theta(x)}{\partial x})
\]

And the other term:

\[
K_{1}+\frac{m^{2}}{1-x^{2}}=\frac{1-x^{2}}{\Theta(\theta)}\frac{\partial^{2}\Theta(x)}{\partial x^{2}}-\frac{x}{\Theta(\theta)}\frac{\partial\Theta(x)}{\partial x}-\frac{x}{\Theta(\theta)}\frac{\partial\Theta(x)}{\partial x}
\]

\[
K_{1}+\frac{m^{2}}{1-x^{2}}=\frac{1-x^{2}}{\Theta(\theta)}\frac{\partial^{2}\Theta(x)}{\partial x^{2}}-\frac{2x}{\Theta(\theta)}\frac{\partial\Theta(x)}{\partial x}
\]

\[
\Theta(\theta)(K_{1}+\frac{m^{2}}{1-x^{2}})=(1-x^{2})\frac{\partial^{2}\Theta(x)}{\partial x^{2}}+-x\frac{\partial\Theta(x)}{\partial x}
\]


\section{P1 Model}

\subsection{How to use:}

\subsubsection{Introduction}

The P1 model is part of spherical harmonics model and it does well
in optically thick medium \cite{Modest2013}.

\part{Bibliography}

\bibliographystyle{naturemag}
\addcontentsline{toc}{section}{\refname}\bibliography{\string"My Collection\string"}

\end{document}
